aneris/examples/transactional_consistency/read_uncommitted/trace/implication_trace.v
@@ -213,7 +213,7 @@ Section trace_proof.
       split_and!; try done.
       eexists T', exec'.
       split_and!; try done.
-      apply extraction_of_add_init_lin; rewrite /is_in_lin_event;
+      apply (extraction_of_add_init_lin tag1); rewrite /is_in_lin_event;
         set_solver.
     }
     iIntros "Htr_is".
@@ -245,7 +245,7 @@ Section trace_proof.
       do 2 (iSplit; first by iPureIntro).
       iSplit; first iPureIntro.
       {
-        apply extraction_of_add_init_lin; rewrite /is_in_lin_event;
+        apply (extraction_of_add_init_lin tag1); rewrite /is_in_lin_event;
         set_solver.
       }
       do 4 (iSplit; first by iPureIntro).
@@ -655,7 +655,7 @@ Section trace_proof.
             destruct Ht''_in as [Ht''_in | Ht''_in]; set_solver.
           * iSplit.
             -- iPureIntro.
-               destruct wo; by apply extraction_of_add1.
+               destruct wo; by apply (extraction_of_add1 _ _ _ _ tag1).
             -- iSplit.
                ++ iPureIntro.
                   apply (valid_transactions_add1 T' (Rd (tag1, c) k wo) c); try done.
@@ -982,7 +982,7 @@ Section trace_proof.
             destruct Ht''_in as [Ht''_in | Ht''_in]; set_solver.
           * iSplit.
             -- iPureIntro.
-               by apply extraction_of_add1.
+               by apply (extraction_of_add1 _ _ _ _ tag1).
             -- iSplit.
                ++ iPureIntro.
                   apply (valid_transactions_add1 T' (Wr (tag1, c) k v) c); try done.
@@ -1274,7 +1274,7 @@ Section trace_proof.
       iSplitR.
       {
         iPureIntro.
-        destruct Hex' as (Hex1 & Hex2 & Hex3).
+        destruct Hex' as (Hex1 & Hex2 & Hex3 & Hex4).
         split.
         - intros le op Hle_in Hlin_le.
           specialize (Hex1 le op).
@@ -1287,12 +1287,15 @@ Section trace_proof.
           + intros trans op Hin_t Hin_op.
             specialize (Hex2 trans op Hin_t Hin_op).
             set_solver.
-          + intros trans op1 op2 Htrans_in Hrel.
-            specialize (Hex3 trans op1 op2 Htrans_in Hrel).
-            destruct Hex3 as (i & j & Hle & Hlookup_i & Hlookup_j).
-            exists i, j.
-            split; first done.
-            split; by apply lookup_app_l_Some.
+          + split. 
+            * intros trans op1 op2 Htrans_in Hrel.
+              specialize (Hex3 trans op1 op2 Htrans_in Hrel).
+              destruct Hex3 as (i & j & Hle & Hlookup_i & Hlookup_j).
+              exists i, j.
+              split; first done.
+              split; by apply lookup_app_l_Some.
+            * intros trans op1 op2 c_trans Ht_in Hop1_in Hop2_in Hcm1 Hcm2 Hconn.
+              apply (next_commit_imp _ _ _ _ _ tag1); try done; set_solver.
       }
       iSplitR; first by iPureIntro.
       iSplitR.
@@ -1684,7 +1687,7 @@ Section trace_proof.
             destruct Ht''_in as [Ht''_in | Ht''_in]; set_solver.
           * iSplit.
             -- iPureIntro.
-               by apply extraction_of_add1.
+               by apply (extraction_of_add1 _ _ _ _ tag1).
             -- iSplit; first by iPureIntro.
                iSplit.
                ++ iDestruct "Htrace_res" as "(%domain & %sub_domain & %tail & Hact_eq & -> & 
